theories_multisorted/LevelOne.v
@@ -1,0 +1,207 @@
+From Prototype Require Import MPrelude MSig.
+
+(** This file defines a generic term grammar with _admissible_ renamings 
+    and substitutions, i.e. renamings are functions [nat -> nat] 
+    and substitutions are functions [nat -> term m].
+    
+    We prove the main properties of substitution and renaming. *)
+
+Module O.
+Section WithSig.
+Context {sig : signature}.
+
+(*********************************************************************************)
+(** *** Level one terms. *)
+(*********************************************************************************)
+
+(** Notations for expressions with known kinds. *)
+#[local] Reserved Notation "'term' m" (at level 0).
+#[local] Reserved Notation "'arg' ty" (at level 0, ty at level 0).
+#[local] Reserved Notation "'args' tys" (at level 0, tys at level 0).
+
+(** Terms over an abstract signature. Terms are indexed by a kind.
+    Note that terms have a sort, but arguments and argument lists
+    can't be assigned a unique sort in general (for instance 
+    what would be the sort of [E_abase _ _] ?). *)
+Inductive expr : kind -> Type :=
+| (** Variable constructor. *)
+  E_var {m} : nat -> term m
+| (** Non-variable constructor applied to a list of arguments. *)
+  E_ctor {m} : forall (c : ctor m), args (ctor_type c) -> term m
+| (** Empty argument list. *)
+  E_al_nil : args []
+| (** Non-empty argument list. *)
+  E_al_cons {ty tys} : arg ty -> args tys -> args (ty :: tys)
+| (** Base argument (e.g. bool or string). *)
+  E_abase : forall b, base_type b -> arg (AT_base b)
+| (** Term argument. *)
+  E_aterm {m} : term m -> arg (AT_term m)
+| (** Binder argument. *)
+  E_abind {ty} : forall m, arg ty -> arg (AT_bind m ty)
+
+where "'term' m" := (expr (Kt m))
+  and "'arg' ty" := (expr (Ka ty))
+  and "'args' tys" := (expr (Kal tys)).
+
+Derive Signature NoConfusion NoConfusionHom for expr.
+
+(*********************************************************************************)
+(** *** Induction on expressions based on their size. *)
+(*********************************************************************************)
+
+(*(** Size of expressions. *)
+Equations expr_size {k} : expr k -> nat :=
+expr_size (E_var _) := 0 ;
+expr_size (E_ctor c al) := S (expr_size al) ;
+expr_size E_al_nil := 0 ;
+expr_size (E_al_cons a al) := S (expr_size a + expr_size al) ;
+expr_size (E_abase _ _) := 0 ;
+expr_size (E_aterm t) := S (expr_size t) ;
+expr_size (E_abind _ a) := S (expr_size a).
+
+Section SizeInd.
+  Context (P : forall k, expr k -> Prop).
+
+  Context (IH : forall s (t : term s), 
+    (forall s' (t' : term s'), expr_size t' < expr_size t -> P s' t') -> 
+    P s t).
+
+  Lemma size_ind : forall s t, P s t.
+  Proof.
+  intros s t. remember (term_size t) as n eqn:E.
+  revert s t E. induction n using Wf_nat.lt_wf_ind. intros s t ->.
+  apply IH. intros s' t' Hlt. eapply H ; eauto.
+  Qed.
+End SizeInd.*)
+
+(** Notation for left to right function composition. *)
+Notation "f >> g" := (fun i => g (f i)) (at level 30).
+
+(*********************************************************************************)
+(** *** Renamings. *)
+(*********************************************************************************)
+
+(** Vector of renamings. *)
+Definition vren := sort -> ren.
+
+(** A vector of identity renamings. *)
+Definition vren_id : vren := fun _ => rid.
+
+(** [vren_shift_point m] has [rshift] at position [m] and [rid] at other positions. *)
+Definition vren_shift_point (m : sort) : vren :=
+  fun m' => if eq_dec m m' then rshift else rid.
+
+(** Lift a vector of renamings through a binder for sort [m]. *)
+Definition vren_up (m : sort) (rv : vren) : vren :=
+  fun m' => if eq_dec m m' then up_ren (rv m') else (rv m').
+
+(** Apply a vector of renamings to an expression. *)
+Equations rename {k} (rv : vren) (t : expr k) : expr k :=
+rename rv (@E_var m i) := E_var (rv m i) ;
+rename rv (E_ctor c al) := E_ctor c (rename rv al) ;
+rename rv E_al_nil := E_al_nil ;
+rename rv (E_al_cons a al) := E_al_cons (rename rv a) (rename rv al) ;
+rename rv (E_abase b x) := E_abase b x ;
+rename rv (E_aterm t) := E_aterm (rename rv t) ;
+rename rv (E_abind m a) := E_abind m (rename (vren_up m rv) a).
+
+(*********************************************************************************)
+(** *** Substitutions. *)
+(*********************************************************************************)
+
+(** A single substitution which yields terms of sort [m]. *)
+Definition subst m := nat -> term m.
+
+(** The identity substitution. *)
+Definition sid {m} : subst m := fun i => E_var i.
+
+(** [sshift] shifts indices by one. *)
+Definition sshift {m} : subst m := 
+  fun i => E_var (S i).
+
+(** Cons a term with a substitution. *)
+Equations scons {m} (t : term m) (s : subst m) : subst m :=
+scons t s 0 := t ;
+scons t s (S i) := s i.
+
+(** Left to right composition of a substitution with a vector of renamings. *)
+Definition srcomp {m} (s : subst m) (r : vren) : subst m := 
+  fun i => rename r (s i).
+
+(** Left to right composition of a renaming with a vector of substitutions. *)
+(*Definition rscomp {m} (r : ren) (s : subst m) : subst m := 
+  fun i => s (r i).*)
+
+(** A vector of substitutions. *)
+Definition vsubst := forall m, subst m.
+
+(** Lift a vector of substitutions through a binder of sort [m].*)
+Definition up_vsubst (m : sort) (svec : vsubst) : vsubst :=
+  let r := vren_shift_point m in 
+  fun m' => 
+    if eq_dec m m' 
+    then scons (E_var 0) (srcomp (svec m') r) 
+    else srcomp (svec m') r.
+
+(** Apply a vector of substitutions to an expression. *)
+Equations substitute {k} (svec : vsubst) (t : expr k) : expr k :=
+substitute svec (@E_var m i) := svec m i ;
+substitute svec (E_ctor c al) := E_ctor c (substitute svec al) ;
+substitute svec E_al_nil := E_al_nil ;
+substitute svec (E_al_cons a al) := E_al_cons (substitute svec a) (substitute svec al) ;
+substitute svec (E_abase b x) := E_abase b x ;
+substitute svec (E_aterm t) := E_aterm (substitute svec t) ;
+substitute svec (E_abind m a) := E_abind m (substitute (up_vsubst m svec) a).
+
+(** Left to right composition of a substitution with a vector of substitutions. *)
+Definition scomp {m} (s : subst m) (svec : vsubst) : subst m :=
+  fun i => substitute svec (s i).
+
+(*********************************************************************************)
+(** *** Setoid Rewrite lemmas. *)
+(*********************************************************************************)
+
+#[export] Instance vren_up_proper : Proper (eq ==> eq2 ==> eq2) vren_up.
+Proof.
+intros m ? <- rv rv' Hrv m' i. unfold vren_up.
+destruct (eq_dec m m').
+- apply up_ren_proper. apply Hrv.
+- now rewrite Hrv. 
+Qed.
+
+#[export] Instance rename_proper k : Proper (eq2 ==> eq ==> eq) (@rename k).
+Proof.
+intros rv rv' Hr t _ <-. induction t in rv, rv', Hr |- * ; simp rename.
+all: try solve [ f_equal ; auto ].
+- now rewrite Hr. 
+- f_equal. apply IHt. now rewrite Hr.
+Qed. 
+
+#[export] Instance substitute_proper k : Proper (eq2 ==> eq ==> eq) (@substitute k).
+
+(*********************************************************************************)
+(** *** Properties of renamings and substitutions. *)
+(*********************************************************************************)
+
+Lemma up_ren_id : up_ren rid =₁ rid.
+Proof. intros [|i] ; reflexivity. Qed.
+
+Lemma vren_up_id m : vren_up m vren_id =₂ vren_id.
+Proof.
+intros m'. unfold vren_up. destruct (eq_dec m m').
+- rewrite up_ren_id. reflexivity.
+- reflexivity.
+Qed.    
+Hint Rewrite vren_up_id : rename.
+
+Lemma rename_id {k} (t : expr k) : 
+  rename vren_id t = t.
+Proof.
+induction t ; simp rename.
+all: now f_equal.
+Qed.
+Hint Rewrite @rename_id : rename.
+
+
+End WithSig.
+End O.
